Clean up the append_log FFI
Append still isn't fully specified, but at least the issues are now
documented.

src/goose_lang/ffi/append_log_ffi.v
@@ -21,6 +21,32 @@ Definition openΣ {ext:ext_op} {Σ: Type} : transition (@state ext (recoverable_
                          | _ => undefined
                          end).
 
+Definition modifyΣ {ext:ext_op} {Σ: Type} (f:Σ -> Σ) : transition (@state ext (recoverable_model Σ)) unit :=
+  bind (reads id) (λ (rs: @state _ (recoverable_model Σ)), match rs.(world) with
+                         | Opened s => modify (set world (fun (_:@ffi_state (recoverable_model Σ)) => Opened (f s)))
+                         | _ => undefined
+                         end).
+
+(* TODO: generalize to a transition to construct the initial value, using a zoom *)
+Definition initTo {ext:ext_op} {Σ: Type} (init:Σ) : transition (@state ext (recoverable_model Σ)) unit :=
+  bind (reads id) (λ (rs: @state _ (recoverable_model Σ)), match rs.(world) with
+                         | UnInit => modify (set world (fun (_:@ffi_state (recoverable_model Σ)) => Opened init))
+                         | _ => undefined
+                         end).
+
+Definition open {ext:ext_op} {Σ: Type} : transition (@state ext (recoverable_model Σ)) Σ :=
+  bind (reads id) (λ (rs: @state _ (recoverable_model Σ)), match rs.(world) with
+                         | Closed s => bind (modify (set world (fun (_:@ffi_state (recoverable_model Σ)) => Opened s)))
+                                      (fun _ => ret s)
+                         | _ => undefined
+                         end).
+
+Definition close {ext:ext_op} {Σ: Type} : transition (RecoverableState Σ) unit :=
+  bind (reads id) (fun s => match s with
+                         | Opened s => modify (fun _ => Closed s)
+                         | _ => undefined
+                         end).
+
 Instance Recoverable_inhabited state : Inhabited (RecoverableState state) := populate UnInit.
 
 Definition ty_ := forall (val_ty:val_types), @ty val_ty.
@@ -47,7 +73,7 @@ Proof.
   solve_countable LogOp_rec 5%nat.
 Qed.
 
-Inductive Log_val := Log (vs:list u8).
+Inductive Log_val := Log (vs:list disk.Block).
 Instance eq_Log_val : EqDecision Log_val.
 Proof.
   solve_decision.
@@ -55,9 +81,10 @@ Defined.
 
 Instance eq_Log_fin : Countable Log_val.
 Proof.
-  refine (inj_countable' (λ v, match v with
+  apply (inj_countable' (λ v, match v with
                                | Log vs => vs
-                               end) Log _); by intros [].
+                               end) Log);
+    by intros [].
 Qed.
 
 Definition log_op : ext_op.
@@ -92,6 +119,23 @@ Section log.
 
   Existing Instances r_mbind r_fmap.
 
+  Definition read_slice (t:ty) (v:val): transition state (list val) :=
+    match v with
+    | PairV (#(LitLoc l)) (PairV #(LitInt sz) #(LitInt cap)) =>
+      (* TODO: implement *)
+      ret []
+    | _ => undefined
+    end.
+
+  Fixpoint tmapM {Σ A B} (f: A -> transition Σ B) (l: list A) : transition Σ (list B) :=
+    match l with
+    | [] => ret []
+    | x::xs => f x;; tmapM f xs
+    end.
+
+  (* TODO: implement *)
+  Definition to_block (l: list val): option disk.Block := None.
+
   Definition log_step (op:LogOp) (v:val) : transition state val :=
     match op, v with
     | GetOp, LitV (LitInt a) =>
@@ -100,10 +144,28 @@ Section log.
       l ← allocateN 4096;
       modify (state_insert_list l (disk.Block_to_vals b));;
       ret $ #(LitLoc l)
+    | ResetOp, LitV LitUnit =>
+      modifyΣ (fun _ => []);;
+      ret $ #()
+    | InitOp, LitV LitUnit =>
+      initTo [];;
+      ret $ ExtV (Log [])
+    | OpenOp, LitV LitUnit =>
+      s ← open;
+      ret $ ExtV (Log s)
+    | AppendOp, v =>
+      (* FIXME: append should be non-atomic in the spec because it needs to read
+         an input slice (and the slices the input points to). *)
+      (* this is absolutely horrendous to reason about *)
+      block_slices ← read_slice (slice.T (slice.T byteT)) v;
+      block_vals ← tmapM (read_slice (@slice.T _ log_ty byteT)) block_slices;
+      new_blocks ← tmapM (unwrap ∘ to_block) block_vals;
+      modifyΣ (λ s, s ++ new_blocks);;
+      ret $ #()
     | _, _ => undefined
     end.
 
   Instance log_semantics : ext_semantics log_op log_model :=
     {| ext_step := log_step;
-       ext_crash := eq; |}.
+       ext_crash := fun s s' => relation.denote close s s' tt; |}.
 End log.
